\documentclass{article}
\title{Anharmonic Group Elements as Generated by Machine}
\author{Ed Rogers}
\date{March 2011}
\begin{document}
   \maketitle
\begin{table}[!hp]
\begin{center}
\begin{tabular}{rcl}
$[-X,H_{0}]$ & = & ${\lambda}^2(6{\cdot}\beta_{21})(B^{6}+A^{6}) + {\lambda}^2(6{\cdot}\beta_{15})(B^{6}-A^{6})$ \\
 & & $ + {\lambda}^2(4{\cdot}\beta_{22})(B^{5}A+BA^{5}) + {\lambda}^2(4{\cdot}\beta_{16})(B^{5}A-BA^{5})$ \\
 & & $ + {\lambda}^2(2{\cdot}\beta_{23})(B^{4}A^{2}+B^{2}A^{4}) + {\lambda}^2(2{\cdot}\beta_{17})(B^{4}A^{2}-B^{2}A^{4})$ \\
 & & $ + {\lambda}(4{\cdot}\beta_{8})(B^{4}+A^{4}) + {\lambda}(4{\cdot}\beta_{5})(B^{4}-A^{4})$ \\
 & & $ + {\lambda}^2(4{\cdot}\beta_{24})(B^{4}+A^{4}) + {\lambda}^2(4{\cdot}\beta_{18})(B^{4}-A^{4})$ \\
 & & $ + {\lambda}(2{\cdot}\beta_{9})(B^{3}A+BA^{3}) + {\lambda}(2{\cdot}\beta_{6})(B^{3}A-BA^{3})$ \\
 & & $ + {\lambda}^2(2{\cdot}\beta_{25})(B^{3}A+BA^{3}) + {\lambda}^2(2{\cdot}\beta_{19})(B^{3}A-BA^{3})$ \\
 & & $ + {\lambda}(2{\cdot}\beta_{10})(B^{2}+A^{2}) + {\lambda}(2{\cdot}\beta_{7})(B^{2}-A^{2})$ \\
 & & $ + {\lambda}^2(2{\cdot}\beta_{26})(B^{2}+A^{2}) + {\lambda}^2(2{\cdot}\beta_{20})(B^{2}-A^{2})$
\end{tabular}
\end{center}
\end{table}

\end{document}
