\documentclass{article}
\title{Anharmonic Group Elements as Generated by Machine}
\author{Ed Rogers}
\date{March 2011}
\begin{document}
   \maketitle
\begin{table}[!hp]
\begin{center}
\begin{tabular}{rcl}
\textbf{Typed in by hand} & & \textbf{Computed by machine} \\
\hline
$[L1,L5]$ = ${\lambda}{\cdot}(4){\cdot}(B^{4}-A^{4})$ \\
\hline
$[L1,L6]$ = ${\lambda}{\cdot}(2){\cdot}(B^{3}A-BA^{3})$ \\
\hline
$[L1,L7]$ = ${\lambda}{\cdot}(2){\cdot}(B^{2}-A^{2})$ \\
\hline
$[L1,L8]$ = ${\lambda}{\cdot}(4){\cdot}(B^{4}+A^{4})$ \\
\hline
$[L1,L9]$ = ${\lambda}{\cdot}(2){\cdot}(B^{3}A+BA^{3})$ \\
\hline
$[L1,L10]$ = ${\lambda}{\cdot}(2){\cdot}(B^{2}+A^{2})$ \\
\hline
$[L3,L5]$ = ${\lambda}^2{\cdot}(4){\cdot}(B^{4}-A^{4})$ \\
\hline
$[L3,L6]$ = ${\lambda}^2{\cdot}(2){\cdot}(B^{3}A-BA^{3})$ \\
\hline
$[L3,L7]$ = ${\lambda}^2{\cdot}(2){\cdot}(B^{2}-A^{2})$ \\
\hline
$[L3,L8]$ = ${\lambda}^2{\cdot}(4){\cdot}(B^{4}+A^{4})$ \\
\hline
$[L3,L9]$ = ${\lambda}^2{\cdot}(2){\cdot}(B^{3}A+BA^{3})$ \\
\hline
$[L3,L10]$ = ${\lambda}^2{\cdot}(2){\cdot}(B^{2}+A^{2})$ \\
\hline
$[L4,L5]$ = ${\lambda}^2{\cdot}(8){\cdot}(B^{5}A-BA^{5}) + {\lambda}^2{\cdot}(12){\cdot}(B^{4}-A^{4})$ \\
\hline
$[L4,L6]$ = ${\lambda}^2{\cdot}(4){\cdot}(B^{4}A^{2}-B^{2}A^{4}) + {\lambda}^2{\cdot}(6){\cdot}(B^{3}A-BA^{3})$ \\
\hline
$[L4,L7]$ = ${\lambda}^2{\cdot}(4){\cdot}(B^{3}A-BA^{3}) + {\lambda}^2{\cdot}(2){\cdot}(B^{2}-A^{2})$ \\
\hline
$[L4,L8]$ = ${\lambda}^2{\cdot}(8){\cdot}(B^{5}A+BA^{5}) + {\lambda}^2{\cdot}(12){\cdot}(B^{4}+A^{4})$ \\
\hline
$[L4,L9]$ = ${\lambda}^2{\cdot}(4){\cdot}(B^{4}A^{2}+B^{2}A^{4}) + {\lambda}^2{\cdot}(6){\cdot}(B^{3}A+BA^{3})$ \\
\hline
$[L4,L10]$ = ${\lambda}^2{\cdot}(4){\cdot}(B^{3}A+BA^{3}) + {\lambda}^2{\cdot}(2){\cdot}(B^{2}+A^{2})$ \\
\hline
$[L5,L6]$ = ${\lambda}^2{\cdot}(-4){\cdot}(B^{6}-A^{6}) + {\lambda}^2{\cdot}(-12){\cdot}(B^{4}A^{2}-B^{2}A^{4}) + {\lambda}^2{\cdot}(-36){\cdot}(B^{3}A-BA^{3}) + {\lambda}^2{\cdot}(-24){\cdot}(B^{2}-A^{2})$ \\
\hline
$[L5,L7]$ = ${\lambda}^2{\cdot}(-8){\cdot}(B^{3}A-BA^{3}) + {\lambda}^2{\cdot}(-12){\cdot}(B^{2}-A^{2})$ \\
\hline
$[L5,L8]$ = ${\lambda}^2{\cdot}(32){\cdot}B^{3}A^{3} + {\lambda}^2{\cdot}(144){\cdot}B^{2}A^{2} + {\lambda}^2{\cdot}(192){\cdot}BA + {\lambda}^2{\cdot}(48)$ \\
\hline
$[L5,L9]$ = ${\lambda}^2{\cdot}(-4){\cdot}(B^{6}+A^{6}) + {\lambda}^2{\cdot}(12){\cdot}(B^{4}A^{2}+B^{2}A^{4}) + {\lambda}^2{\cdot}(36){\cdot}(B^{3}A+BA^{3}) + {\lambda}^2{\cdot}(24){\cdot}(B^{2}+A^{2})$ \\
\hline
$[L5,L10]$ = ${\lambda}^2{\cdot}(8){\cdot}(B^{3}A+BA^{3}) + {\lambda}^2{\cdot}(12){\cdot}(B^{2}+A^{2})$ \\
\hline
$[L6,L7]$ = ${\lambda}^2{\cdot}(2){\cdot}(B^{4}-A^{4})$ \\
\hline
$[L6,L8]$ = ${\lambda}^2{\cdot}(4){\cdot}(B^{6}+A^{6}) + {\lambda}^2{\cdot}(12){\cdot}(B^{4}A^{2}+B^{2}A^{4}) + {\lambda}^2{\cdot}(36){\cdot}(B^{3}A+BA^{3}) + {\lambda}^2{\cdot}(24){\cdot}(B^{2}+A^{2})$ \\
\hline
$[L6,L9]$ = ${\lambda}^2{\cdot}(16){\cdot}B^{3}A^{3} + {\lambda}^2{\cdot}(36){\cdot}B^{2}A^{2} + {\lambda}^2{\cdot}(12){\cdot}BA$ \\
\hline
$[L6,L10]$ = ${\lambda}^2{\cdot}(2){\cdot}(B^{4}+A^{4}) + {\lambda}^2{\cdot}(12){\cdot}B^{2}A^{2} + {\lambda}^2{\cdot}(12){\cdot}BA$ \\
\hline
$[L7,L8]$ = ${\lambda}^2{\cdot}(8){\cdot}(B^{3}A+BA^{3}) + {\lambda}^2{\cdot}(12){\cdot}(B^{2}+A^{2})$ \\
\hline
$[L7,L9]$ = ${\lambda}^2{\cdot}(-2){\cdot}(B^{4}+A^{4}) + {\lambda}^2{\cdot}(12){\cdot}B^{2}A^{2} + {\lambda}^2{\cdot}(12){\cdot}BA$ \\
\hline
$[L7,L10]$ = ${\lambda}^2{\cdot}(8){\cdot}BA + {\lambda}^2{\cdot}(4)$ \\
\hline
$[L8,L9]$ = ${\lambda}^2{\cdot}(-4){\cdot}(B^{6}-A^{6}) + {\lambda}^2{\cdot}(12){\cdot}(B^{4}A^{2}-B^{2}A^{4}) + {\lambda}^2{\cdot}(36){\cdot}(B^{3}A-BA^{3}) + {\lambda}^2{\cdot}(24){\cdot}(B^{2}-A^{2})$ \\
\hline
$[L8,L10]$ = ${\lambda}^2{\cdot}(8){\cdot}(B^{3}A-BA^{3}) + {\lambda}^2{\cdot}(12){\cdot}(B^{2}-A^{2})$ \\
\hline
$[L9,L10]$ = ${\lambda}^2{\cdot}(2){\cdot}(B^{4}-A^{4})$ \\
\hline
\end{tabular}
\end{center}
\end{table}

\end{document}
